new_proof/RefinementDenotationProp.v
@@ -69,12 +69,14 @@ Qed.
 
 Global Hint Constructors ok_dctx: core.
 
-Ltac refinement_solver7 :=
-  listctx_set_simpl4;
-  match goal with
-  | [H: {_;_;_}⟦_⟧ ?e |- _ ∉ fv_tm ?e] =>
-      apply rR_regular1 in H; mydestr; basic_typing_solver
-  end || refinement_solver6.
+(* refine *)
+
+(* Ltac refinement_solver7 := *)
+(*   listctx_set_simpl4; *)
+(*   match goal with *)
+(*   | [H: {_;_;_}⟦_⟧ ?e |- _ ∉ fv_tm ?e] => *)
+(*       apply rR_regular1 in H; mydestr; basic_typing_solver *)
+(*   end || refinement_solver6. *)
 
 (* Lemma reduction_tmeet_iff_both: forall (T: base_ty) e1 e2, *)
 (*     [] ⊢t e1 ⋮t T -> [] ⊢t e2 ⋮t T -> (forall (v: value), (mk_term_meet T e1 e2) ↪* v <-> e1 ↪* v /\ e2 ↪* v). *)
@@ -155,11 +157,17 @@ Proof.
     rewrite subst_fresh_tm.
     rewrite rR_shadow_update_st_c; refinement_solver.
     refinement_solver7. basic_typing_solver7. set_solver.
-  - constructor; refinement_solver7.
-    mydestr.
-    exists x; split; auto. intros. apply IHΓ; eauto.
-    rewrite rR_shadow_update_st; refinement_solver.
-        eapply termR_perserve_rR; eauto; refinement_solver5.
+  - destruct (decide (is_arr r)).
+    + apply ctxrR_cons_under_arr; refinement_solver7. mydestr.
+      exists x; split; auto. intros. apply IHΓ; eauto.
+      rewrite rR_shadow_update_st; refinement_solver.
+      eapply termR_perserve_rR; eauto; refinement_solver5.
+      eapply termR_tlete_drop_halt_lhs'; refinement_solver7.
+    + constructor; refinement_solver7.
+      mydestr.
+      exists x; split; auto. intros. apply IHΓ; eauto.
+      rewrite rR_shadow_update_st; refinement_solver.
+      eapply termR_perserve_rR; eauto; refinement_solver5.
       eapply termR_tlete_drop_halt_lhs'; refinement_solver7.
 Qed.
 
@@ -191,7 +199,7 @@ Proof.
     assert ({0;b∅;st}⟦r⟧ (random_inhabitant r)).
     apply random_inhabitant_in_any_under; refinement_solver7.
     split; auto. intros.
-    assert ([] ⊢t v_x ⋮v ⌊r⌋). refinement_solver7.
+    assert ([] ⊢t v_x ⋮v ⌊r⌋) by refinement_solver7.
     assert (closed_value v_x) as Hclosedv. basic_typing_solver.
     apply state_insert_closed_value with (a:=a) (st:=st) in Hclosedv.
     destruct Hclosedv; mydestr; subst.
@@ -243,6 +251,8 @@ Ltac auto_ty_exfalso4 :=
   auto_ty_exfalso3;
   match goal with
   | [H: is_arr [v:_|_|_|_] |- _ ] =>invclear H
+  | [H: is_arr {v:_|_|_|_} |- _ ] =>invclear H
+  | [H: {v:_|_|_|_} = [v:_|_|_|_]|- _] => invclear H
   end.
 
 Lemma rRctx_pre_weakening: forall Γ1 Γ2 st τ,
@@ -252,25 +262,151 @@ Lemma rRctx_pre_weakening: forall Γ1 Γ2 st τ,
 Proof.
   induction Γ1; intros; RD_simp; denotation_simp.
   - apply rRctx_pre_weakening_empty; auto.
-  - invclear H0.
-    + invclear H1; auto_ty_exfalso. constructor; refinement_solver5.
-      listctx_set_simpl4. refinement_solver7.
-      ctx_erase_simp. basic_typing_solver7. ctx_erase_simp5.
-    + destruct (classic (is_arr r)); auto_ty_exfalso.
-      { invclear H1; auto_ty_exfalso. invclear H7; try auto_ty_exfalso4.
-        constructor; refinement_solver7.
-        ctx_erase_simp. basic_typing_solver7. refinement_solver7.
-        is_arr_simp. }
-      { invclear H1; auto_ty_exfalso. invclear H7; auto_ty_exfalso.
-        constructor; refinement_solver7.
-        ctx_erase_simp. basic_typing_solver7. refinement_solver7.
-        exists (x4 ⊗{ x0 } x). split. eapply rR_tmeet_when_both; auto. intros.
-        rewrite reduction_tmeet_iff_both in H6; refinement_solver7; mydestr; eauto. }
+  - invclear H1; invclear H0; try auto_ty_exfalso4.
+    + constructor; refinement_solver. basic_typing_solver7. ctx_erase_simp5.
+    + denotation_simp. invclear H9; auto_ty_exfalso.
+      constructor; auto. refinement_solver. ctx_erase_simp5. basic_typing_solver7. ctx_erase_simp5.
+      exists (x0 ⊗{ x1 } x). split. eapply rR_tmeet_when_both; auto. intros.
+      rewrite reduction_tmeet_iff_both in H6; refinement_solver7; mydestr; eauto.
+    + invclear H9; try auto_ty_exfalso4. apply ctxrR_cons_under_arr; auto.
+      denotation_simp. refinement_solver.
+      ctx_erase_simp. basic_typing_solver7. refinement_solver.
+      is_arr_simp.
 Qed.
+
+Check ok_first_not_equal_hd.
+
+Lemma basic_type_first_not_equal_hd_tm
+     : ∀ (Γ : list (atom * ty)) (x y : atom) (a b : ty) e T, ((x, a) :: Γ ++ [(y, b)]) ⊢t e ⋮t T → x ≠ y.
+Proof.
+  intros. assert (ok ((x, a) :: Γ ++ [(y, b)])) by basic_typing_solver2.
+  eapply ok_first_not_equal_hd; eauto.
+Qed.
+
+Lemma basic_type_first_not_equal_hd_value
+     : ∀ (Γ : list (atom * ty)) (x y : atom) (a b : ty) e T, ((x, a) :: Γ ++ [(y, b)]) ⊢t e ⋮v T → x ≠ y.
+Proof.
+  intros. assert (ok ((x, a) :: Γ ++ [(y, b)])) by basic_typing_solver2.
+  eapply ok_first_not_equal_hd; eauto.
+Qed.
+
+Ltac basic_typing_solver8 :=
+  match goal with
+  | [H: ((?x, _) :: _ ++ [(?y, _)]) ⊢t _ ⋮t _ |- ?x ≠ ?y] => apply basic_type_first_not_equal_hd_tm in H; auto
+  | [H: ((?x, _) :: _ ++ [(?y, _)]) ⊢t _ ⋮v _ |- ?x ≠ ?y] => apply basic_type_first_not_equal_hd_value in H; auto
+  end || basic_typing_solver7.
+
+Lemma wf_implies_ctxrR_tlete: forall Γ st x b n d ϕ e_x e τ,
+    not_overbasety τ -> not_overbasety τ_x ->
+    wf_ctxrR st (Γ ++ [(x, τ_x)]) ->
+    {st}⟦mk_eq_var ty⟧{Γ ++ [(x, τ_x)] } e_x ->
+    {st}⟦τ⟧{Γ ++ [(x, τ_x)] } e ->
+    {st}⟦τ⟧{Γ ++ [(x, τ_x)] } (tlete e_x e).
+Proof.
+
+Lemma wf_implies_ctxrR_tlete: forall Γ st x τ_x e_x e τ,
+    not_overbasety τ -> not_overbasety τ_x ->
+    wf_ctxrR st (Γ ++ [(x, τ_x)]) ->
+    {st}⟦mk_eq_var ty⟧{Γ ++ [(x, τ_x)] } e_x ->
+    {st}⟦τ⟧{Γ ++ [(x, τ_x)] } e ->
+    {st}⟦τ⟧{Γ ++ [(x, τ_x)] } (tlete e_x e).
+Proof.
+  induction Γ; intros; mydestr; RD_simp; denotation_simp.
+  - invclear H3. invclear H0.
+    + mydestr. invclear H1; try auto_ty_exfalso.
+      denotation_simp. constructor; auto. admit.
+      exists x0. split; auto. intros. eapply H3 in H6; eauto. RD_simp; auto. admit.
+    + invclear H1. auto_ty_exfalso.
+      apply ctxrR_cons_under_arr; auto. admit.
+      is_arr_simp. intros. apply H14 in H1. RD_simp; auto. admit.
+  - invclear H2; invclear H3; try auto_ty_exfalso4.
+    + invclear H1; try auto_ty_exfalso4; ctx_erase_simp.
+      constructor; auto. admit.
+      intros.
+      specialize (H13 _ H1). specialize (H19 _ H1). specialize (H14 _ H1).
+      eapply IHΓ in H19; eauto.
+    + denotation_simp. invclear H1. constructor; auto. denotation_simp. refinement_solver. admit.
+      mydestr.
+      exists ((x0 ⊗{ x6 } x1) ⊗{ x6 } x2).
+      split. apply rR_tmeet3_when_all; auto.
+      intros. rewrite reduction_tmeet3_iff_all in H13; refinement_solver7; mydestr.
+      assert (wf_ctxrR (({a↦v_x}) st) (Γ ++ [(x, τ_x)])) as Hwf by eauto.
+      assert ({({a↦v_x}) st}⟦τ_x⟧{Γ} (tlete e_x0 (a \t\ e_x))) as Hex by eauto.
+      assert (({({a↦v_x}) st}⟦τ⟧{Γ ++ [(x, τ_x)] }) (tlete e_x0 (a \t\ e))) as He by eauto.
+      assert ([] ⊢t v_x ⋮v x6). refinement_solver7. denotation_simp.
+      eapply IHΓ in He; eauto.
+      eapply termR_perserve_ctxrR; refinement_solver7.
+      eapply termR_tlete_commute_tlete; eauto; refinement_solver.
+      basic_typing_solver8.
+
+      admit. denotation_simp. refinement_solver7.
+    + apply ctxrR_cons_under_arr; auto. denotation_simp. eapply let_store_typable; eauto.
+      is_arr_simp. intros.
+      specialize (H23 _ H2). specialize (H19 _ H2). specialize (H13 _ H2).
+      (* assert ([] ⊢t e_x ⋮t ⌊τ_x⌋) as Hxx by refinement_solver. *)
+      eapply IHΓ in H23; eauto. eauto.
+      assert (({st}⟦τ⟧{Γ}) (tlete e_x (x \t\ (tlete e_x0 (a \t\ e))))). {  eapply IHΓ in H23; eauto.
+      eapply IHΓ in H23; eauto.
+      eapply termR_perserve_ctxrR; refinement_solver7.
+      eapply termR_tlete_commute_tlete; eauto; refinement_solver.
+      basic_typing_solver8. admit.
+      denotation_simp.
+Admitted.
+
+
+
+Lemma wf_implies_ctxrR_tlete: forall Γ st x τ_x e_x e τ,
+    not_overbasety τ -> not_overbasety τ_x ->
+    wf_ctxrR st (Γ ++ [(x, τ_x)]) ->
+    {st}⟦τ_x⟧{Γ} e_x ->
+    {st}⟦τ⟧{Γ ++ [(x, τ_x)] } e ->
+    {st}⟦τ⟧{Γ ++ [(x, τ_x)] } (tlete e_x e).
+Proof.
+  induction Γ; intros; mydestr; RD_simp; denotation_simp.
+  - invclear H3. invclear H0.
+    + mydestr. invclear H1; try auto_ty_exfalso.
+      denotation_simp. constructor; auto. admit.
+      exists x0. split; auto. intros. eapply H3 in H6; eauto. RD_simp; auto. admit.
+    + invclear H1. auto_ty_exfalso.
+      apply ctxrR_cons_under_arr; auto. admit.
+      is_arr_simp. intros. apply H14 in H1. RD_simp; auto. admit.
+  - invclear H2; invclear H3; try auto_ty_exfalso4.
+    + invclear H1; try auto_ty_exfalso4; ctx_erase_simp.
+      constructor; auto. admit.
+      intros.
+      specialize (H13 _ H1). specialize (H19 _ H1). specialize (H14 _ H1).
+      eapply IHΓ in H19; eauto.
+    + denotation_simp. invclear H1. constructor; auto. denotation_simp. refinement_solver. admit.
+      mydestr.
+      exists ((x0 ⊗{ x6 } x1) ⊗{ x6 } x2).
+      split. apply rR_tmeet3_when_all; auto.
+      intros. rewrite reduction_tmeet3_iff_all in H13; refinement_solver7; mydestr.
+      assert (wf_ctxrR (({a↦v_x}) st) (Γ ++ [(x, τ_x)])) as Hwf by eauto.
+      assert ({({a↦v_x}) st}⟦τ_x⟧{Γ} (tlete e_x0 (a \t\ e_x))) as Hex by eauto.
+      assert (({({a↦v_x}) st}⟦τ⟧{Γ ++ [(x, τ_x)] }) (tlete e_x0 (a \t\ e))) as He by eauto.
+      assert ([] ⊢t v_x ⋮v x6). refinement_solver7. denotation_simp.
+      eapply IHΓ in He; eauto.
+      eapply termR_perserve_ctxrR; refinement_solver7.
+      eapply termR_tlete_commute_tlete; eauto; refinement_solver.
+      basic_typing_solver8.
+
+      admit. denotation_simp. refinement_solver7.
+    + apply ctxrR_cons_under_arr; auto. denotation_simp. eapply let_store_typable; eauto.
+      is_arr_simp. intros.
+      specialize (H23 _ H2). specialize (H19 _ H2). specialize (H13 _ H2).
+      (* assert ([] ⊢t e_x ⋮t ⌊τ_x⌋) as Hxx by refinement_solver. *)
+      eapply IHΓ in H23; eauto. eauto.
+      assert (({st}⟦τ⟧{Γ}) (tlete e_x (x \t\ (tlete e_x0 (a \t\ e))))). {  eapply IHΓ in H23; eauto.
+      eapply IHΓ in H23; eauto.
+      eapply termR_perserve_ctxrR; refinement_solver7.
+      eapply termR_tlete_commute_tlete; eauto; refinement_solver.
+      basic_typing_solver8. admit.
+      denotation_simp.
+Admitted.
 
 Lemma wf_implies_ctxrR_drop_last: forall Γ st x τ_x e_x e τ,
     not_overbasety τ -> not_overbasety τ_x ->
-    closed_rty 0 (ctxdom Γ ∪ dom _ st) τ ->
+    closed_rty 0 (ctxdom ⦑Γ⦒ ∪ dom _ st) τ ->
     wf_ctxrR st (Γ ++ [(x, τ_x)]) ->
     x ∉ stale τ ->
     {st}⟦τ_x⟧{Γ} e_x ->
@@ -278,76 +414,43 @@ Lemma wf_implies_ctxrR_drop_last: forall Γ st x τ_x e_x e τ,
     {st}⟦τ⟧{Γ} (tlete e_x (x \t\ e)).
 Proof.
   induction Γ; intros; mydestr; RD_simp; denotation_simp.
-  - invclear H2; invclear H5; auto_ty_exfalso. mydestr.
-    apply H12 in H2; mydestr.
-    eapply H4 in H6; eauto. RD_simp.
-    rewrite rR_shadow_update_st in H13; auto.
-    refinement_solver.
-  - invclear H2; invclear H4; invclear H5; auto_ty_exfalso; ctx_erase_simp.
+  - invclear H2; invclear H5; try auto_ty_exfalso4.
+    + denotation_simp. apply H12 in H2; mydestr. eapply H4 in H6; eauto. RD_simp.
+      rewrite rR_shadow_update_st in H10; auto.
+      refinement_solver.
+    + is_arr_simp. apply H19 in H6. RD_simp; auto.
+  - invclear H2; invclear H4; invclear H5; try auto_ty_exfalso4; ctx_erase_simp.
     + invclear H9; auto_ty_exfalso. constructor; auto. eapply let_store_typable; eauto.
       intros.
       assert (wf_ctxrR (<[a:=c_x]> st) (Γ ++ [(x, τ_x)])) by auto.
       assert (({<[a:=c_x]> st}⟦τ_x⟧{Γ}) ({a := c_x }t e_x)) by auto.
       apply H22 in H2.
-      (* assert (({a := c_x }t (e ^t^ x)) = ({a := c_x }t e) ^t^ x) as Htmp. admit. *)
-      (* rewrite Htmp in H2. clear Htmp. *)
       eapply IHΓ in H2; eauto. simpl.
       rewrite subst_close_tm in H2; auto; refinement_solver7. refinement_solver.
-    + constructor; auto. eapply let_store_typable; eauto.
-      destruct (classic (is_arr r)).
-      { is_arr_simp. intros.
-        specialize (H23 _ H4). specialize (H19 _ H4). specialize (H13 _ H4).
-        eapply IHΓ in H23; eauto. admit. admit. }
-      { mydestr; auto_ty_exfalso.
-        exists ((x0 ⊗{ x3 } x1) ⊗{ x3 } x2).
-        split. apply rR_tmeet3_when_all; auto.
-        intros. rewrite reduction_tmeet3_iff_all in H7; refinement_solver7; mydestr.
-        assert (wf_ctxrR (({a↦v_x}) st) (Γ ++ [(x, τ_x)])) as Hwf by eauto.
-        assert ({({a↦v_x}) st}⟦τ_x⟧{Γ} (tlete e_x0 (a \t\ e_x))) as Hex by eauto.
-        assert (({({a↦v_x}) st}⟦τ⟧{Γ ++ [(x, τ_x)] }) (tlete e_x0 (a \t\ e))) as He by eauto.
-        assert ([] ⊢t v_x ⋮v x3). refinement_solver7.
-        assert (closed_value v_x) as Hclosedv. basic_typing_solver.
-        apply state_insert_closed_value with (a:=a) (st:=st) in Hclosedv.
-        destruct Hclosedv; mydestr; subst.
-        eapply IHΓ in He; eauto. admit.
-        assert (dom aset (({a↦x7}) st) ≡ {[a]} ∪ dom aset st)
-        by (eapply insert_constant_in_st; refinement_solver7).
-        refinement_solver7.
-        admit.
-      }
+    + constructor; auto. denotation_simp. eapply let_store_typable; eauto.
+      mydestr; auto_ty_exfalso.
+      exists ((x0 ⊗{ x3 } x1) ⊗{ x3 } x2).
+      split. apply rR_tmeet3_when_all; auto.
+      intros. rewrite reduction_tmeet3_iff_all in H15; refinement_solver7; mydestr.
+      assert (wf_ctxrR (({a↦v_x}) st) (Γ ++ [(x, τ_x)])) as Hwf by eauto.
+      assert ({({a↦v_x}) st}⟦τ_x⟧{Γ} (tlete e_x0 (a \t\ e_x))) as Hex by eauto.
+      assert (({({a↦v_x}) st}⟦τ⟧{Γ ++ [(x, τ_x)] }) (tlete e_x0 (a \t\ e))) as He by eauto.
+      assert ([] ⊢t v_x ⋮v x3). refinement_solver7. denotation_simp.
+      eapply IHΓ in He; eauto.
+      eapply termR_perserve_ctxrR; refinement_solver7.
+      eapply termR_tlete_commute_tlete; eauto; refinement_solver.
+      basic_typing_solver8.
+
+      admit. denotation_simp. refinement_solver7.
+    + apply ctxrR_cons_under_arr; auto. denotation_simp. eapply let_store_typable; eauto.
+      is_arr_simp. intros.
+      specialize (H23 _ H2). specialize (H19 _ H2). specialize (H13 _ H2).
+      (* assert ([] ⊢t e_x ⋮t ⌊τ_x⌋) as Hxx by refinement_solver. *)
+      eapply IHΓ in H23; eauto. eauto.
+      assert (({st}⟦τ⟧{Γ}) (tlete e_x (x \t\ (tlete e_x0 (a \t\ e))))). {  eapply IHΓ in H23; eauto.
+      eapply IHΓ in H23; eauto.
+      eapply termR_perserve_ctxrR; refinement_solver7.
+      eapply termR_tlete_commute_tlete; eauto; refinement_solver.
+      basic_typing_solver8. admit.
+      denotation_simp.
 Admitted.
-
-
-(*       assert (({st}⟦τ⟧{Γ}) (tlete (tlete e_x0 (a \t\ e_x)) (x \t\ tlete e_x0 (a \t\ e)))). *)
-(*       eapply IHΓ; eauto. admit. *)
-(*       eapply IHΓ in H23; eauto. admit. *)
-(*       refinement_solver7. *)
-
-
-
-(*       constructor; auto. eapply let_store_typable; eauto. *)
-(*       exists ((x0 ⊗{  ⌊r⌋ } x1) ⊗{ ⌊r⌋ } x2). *)
-(*       split. apply rR_tmeet3_when_all; auto. *)
-(*       intros. rewrite reduction_tmeet3_iff_all in H20; refinement_solver7; mydestr. *)
-(*       assert (wf_ctxrR (({a↦v_x}) st) (Γ ++ [(x, τ_x)])) as Hwf by eauto. *)
-(*       assert ({({a↦v_x}) st}⟦τ_x⟧{Γ} (tlete e_x0 (a \t\ e_x))) as Hex by eauto. *)
-(*       assert (({({a↦v_x}) st}⟦τ⟧{Γ ++ [(x, τ_x)] }) (tlete e_x0 (a \t\ e))) as He by eauto. *)
-(*       assert ([] ⊢t v_x ⋮v ⌊r⌋). refinement_solver7. *)
-(*       assert (closed_value v_x) as Hclosedv. basic_typing_solver. *)
-(*       apply state_insert_closed_value with (a:=a) (st:=st) in Hclosedv. *)
-(*       destruct Hclosedv; mydestr; subst. *)
-(*       { eapply IHΓ in He; eauto. admit. *)
-(*         assert (dom aset (({a↦x3}) st) ≡ {[a]} ∪ dom aset st) *)
-(*         by (eapply insert_constant_in_st; refinement_solver7). *)
-(*         refinement_solver7. *)
-(*       } *)
-(*       { rename H25 into Hzz. *)
-(*         rewrite Hzz in He. rewrite Hzz. rewrite Hzz in Hex. rewrite Hzz in Hwf. *)
-(*         ctx_erase_simp. *)
-(*         assert (ok ((a, ⌊r⌋) :: ⌊Γ⌋* ++ ⌊[(x, τ_x)]⌋) as Hok by basic_typing_solver. *)
-(*         assert (a <> x). listctx_set_solver. *)
-(*         eapply IHΓ in He; eauto. admit. *)
-(*         apply closed_rty_cap with *)
-(*           (d1:= (ctxdom Γ ∪ ({[x]} ∪ ∅) ∪ dom aset st)) *)
-(*           (d2:= ({[a]} ∪ ctxdom Γ ∪ dom aset st)); eauto; refinement_solver7. } *)
-(* Admitted. *)
